-Extraction is now more stable: For computable/computableTime, we always infer the TT-argument before we infer the term itself. This fixes occasional bugs when infering (extracted _). -Extraction now is able to treat projections out of Record better, i.e. we can project a function out of a record and add a hint, see for example Synthetic.v decInTime -Most Complexity-related predicates are now records in Type, to allow projections -Proofs for NP hardness/Completeness of GenNP and GenNPHalt are now more straightforward -Relations for definition of NP-completeness are now own predicate  Furthermore, we require that it is soudn for all certificates and that there always is a small certificate -added proofs to allow switching to computable time bounds in many cases

theories/L/Complexity/NP.v
@@ -19,41 +19,67 @@ Section NP_certificate_fix.
   Context `{RegY : registered Y}.
 
   Definition inTimePoly {X} `{registered X} `(P:restrictedP vX):=
-    exists f, decInTime P f /\ inOPoly f /\ monotonic f.
+    exists f, inhabited (decInTime P f) /\ inOPoly f /\ monotonic f.
 
-  Local Set Warnings "-cannot-define-projection".
-  
-  Record polyCertRel {vX : X -> Prop} (P:restrictedP vX) (R: {x | vX x} -> Y -> Prop) :Prop :=
+  Record polyCertRel {vX : X -> Prop} (P:restrictedP vX) (R: {x | vX x} -> Y -> Prop) : Type :=
     polyBoundedWitness_introSpec
       {
-        p : nat -> nat;
-        polyCertRel_sound : forall x y, R x y -> P x;
-        polyCertRel_complete : forall x, P x -> exists (y:Y), R x y /\ size (enc y) <= p (size (enc (proj1_sig x)));
-        poly__p : inOPoly p ;
-        mono__p : monotonic p;
+        p__pCR : nat -> nat;
+        sound__pCR : forall x y, R x y -> P x;
+        complete__pCR : forall x, P x -> exists (y:Y), R x y /\ size (enc y) <= p__pCR (size (enc (proj1_sig x)));
+        poly__pCR : inOPoly p__pCR ;
+        mono__pCR : monotonic p__pCR;
       }.
 
+  Lemma polyCertRel_compPoly vX (P:restrictedP vX) R:
+    polyCertRel P R -> exists H : polyCertRel P R , inhabited (polyTimeComputable (p__pCR H)).
+  Proof.
+    intros R__spec.  destruct (inOPoly_computable (poly__pCR R__spec)) as (p'&?&Hbounds&?&?).
+    unshelve eexists.
+    exists p'.
+    3-5:assumption.
+    now apply sound__pCR.
+    intros ? H'. edestruct (complete__pCR R__spec H') as (y&?&H'').
+    do 2 esplit. easy.
+    rewrite H'',Hbounds. easy.
+  Qed.
+
+  
+  Lemma inTimePoly_compTime  `(P:restrictedP (X:=X) vX):
+    inTimePoly P -> exists f, inhabited (polyTimeComputable f) /\ inhabited (decInTime P f) /\ inOPoly f /\ monotonic f.
+  Proof.
+    intros (time&[P__dec]&t__poly&t__mono).
+    destruct (inOPoly_computable t__poly) as (p'&?&Hbounds&?&?).
+    exists p'. repeat apply conj. 1,3,4:easy.
+    split.
+    eexists. 2:exact (correct__decInTime P__dec).
+    eexists. eapply computesTime_timeLeq. 2:now apply extTCorrect.
+    repeat intro;cbn [fst snd]. now rewrite Hbounds.
+  Qed.
+
+  (*
   Lemma polyCertRel_equiv {vX : X -> Prop} (P P' : restrictedP vX) R :
     (forall x, P x <-> P' x)
-    -> polyCertRel P R <-> polyCertRel P' R.
+    -> polyCertRel P R -> polyCertRel P' R.
   Proof.
     intros H. split;intros[].
-    all:eexists;try eassumption.
-    1,2:setoid_rewrite <- H.
-    3,4:setoid_rewrite H. all:easy.
-  Qed.
+    all:eexists;try eassumption;intros x. all:specialize (H x).
+    all:firstorder.
+  Qed.*)
 
   (*TODO: here and below, specify the lemmas using restrictBy, as this is main intend in use. *)
   
 End NP_certificate_fix.
+Smpl Add 10 (simple apply poly__pCR) : inO.
+Smpl Add 10 (simple apply mono__pCR) : inO.
 
 Local Set Warnings "-cannot-define-projection".
 Record inNP {X} `{registered X} `(P:restrictedP (X:=X) vX) : Prop :=
   inNP_introSpec
     {
-      R : {x | vX x} -> term -> Prop; (* certificate fixed to term for simplicity *)
-      poly__R : inTimePoly (curryRestrRel R);
-      R__correct : polyCertRel P R; (*TODO: What if moved to spec__R(better: move condition externally)? and only require that some small certificate satisfies condition? It seems that we might want that every certificate is valid, but there must exist a small one? *)
+      R_NP : {x | vX x} -> term -> Prop; (* certificate fixed to term for simplicity *)
+      R_NP__comp : inTimePoly (curryRestrRel R_NP);
+      R_NP__correct : polyCertRel P (R_NP) (*TODO: What if moved to spec__R(better: move condition externally)? and only require that some small certificate satisfies condition? It seems that we might want that every certificate is valid, but there must exist a small one? *)
     }.
 
 
@@ -65,43 +91,42 @@ Lemma inNP_intro {X Y} `{_:registered X} `{registered Y} {_:decodable Y} `(P:@re
   -> inTimePoly (curryRestrRel R)
   -> polyCertRel P R
   -> inNP P.
-Proof. cbn.
-  intros decode__comp poly_R bal_R.
+Proof.
+  cbn.
+  intros decode__comp R__comp R__bound.
   eexists (fun x y => exists y', y = enc y' /\ R x y').
-  2:{ destruct bal_R as [? ? ? ? ?].
-      exists (fun x => p x * 11).
-      3,4:now smpl_inO.
-      -intros x y' (y&->&Hy). eauto.
-      -intros x ?. edestruct polyCertRel_complete as (y&?&?). easy.
+  2:{ 
+      exists (fun x => p__pCR R__bound x * 11).
+      3,4:solve [smpl_inO].
+      -intros x y' (y&->&Hy). now eapply sound__pCR.
+      -intros x ?. edestruct (complete__pCR R__bound) as (y&?&?). easy.
        exists (enc y);split. easy.
        rewrite size_term_enc. lia.
   }
-  { destruct poly_R as (t__f&[f [] ?]&?&mono_t__f).
-    destruct decode__comp as [? [] ? ? ?].
+  { (*TODO: simplify*)
+    destruct R__comp as (t__f&[R__comp]&?&mono_t__f).
     pose (f' (x:X*term) :=
             let '(x,y):= x in
             match decode Y y with
               None => false
-            | Some y => f (x,y)
+            | Some y => (f__decInTime R__comp) (x,y)
             end).
     evar (t__f' : nat -> nat). [t__f']:intro.
-    exists t__f'. repeat eapply conj.
-    -exists f'. split.
-     +unfold f'. extract. solverec.
+    exists t__f'. repeat eapply conj. 
+    -split. exists f'. 
+     +unfold f'. extract.
+      solverec.
       all:rewrite !size_prod. all:cbn [fst snd].
-      all:hnf in polyTimeC__mono,mono_t__f.
       *eapply decode_correct2 in H2 as <-.
-
-
        remember (size (enc a) + size (enc (enc y)) + 4) as n eqn:eqn.
-       rewrite mono_t__f with (x':=n). 2:subst n;rewrite <- size_term_enc_r;lia.
-       rewrite polyTimeC__mono with (x':=n). 2:lia.
+       rewrite (mono_t__f _ n). 2:subst n;rewrite <- size_term_enc_r;lia.
+       rewrite (mono__polyTC _ (x':=n)). 2:lia.
        unfold t__f';reflexivity.
-      *rewrite polyTimeC__mono with (x':=(size (enc a) + size (enc b) + 4)). 2:lia.
+      *rewrite (mono__polyTC _ (x':=(size (enc a) + size (enc b) + 4))). 2:lia.
        unfold t__f'. lia.
      +unfold f'. intros [x] Hx. cbn.
       destruct decode  as [y| ] eqn:H'.
-      *etransitivity. 2:unshelve eapply decInTime_correct;easy. cbn.
+      *etransitivity. 2:unshelve eapply correct__decInTime;easy. cbn.
        eapply decode_correct2 in H'. symmetry in H'.
        split;[intros (y'&?&?)|intros ?].
        --cbn. enough (y = y') by congruence. eapply inj_enc. congruence.
@@ -135,9 +160,18 @@ Proof.
   intros H H'. econstructor. eassumption. all:intros ? ?. apply (proj2_sig (H' _ Hx)).
 Qed.
 
-Lemma reducesPolyMO_elimCompact X Y `{RX: registered X} `{RY:registered Y} `(P : restrictedP vX) `(Q : restrictedP vY):
+
+Lemma reducesPolyMO_intro_restrictBy X Y `{RX: registered X} `{RY:registered Y} (vP P : X -> Prop) (vQ Q:Y->Prop) (f:X -> Y):
+  polyTimeComputable f
+  -> (forall x (Hx : vP x), {Hfx : vQ (f x) | (P x <-> Q (f x))})
+  -> restrictBy vP P ⪯p restrictBy vQ Q.
+Proof.
+  intros H H'. econstructor. eassumption. Unshelve. all:intros ? ?. all:now edestruct H'. 
+Qed.
+
+Lemma reducesPolyMO_elim X Y `{RX: registered X} `{RY:registered Y} `(P : restrictedP vX) `(Q : restrictedP vY):
   P ⪯p Q ->
-  exists f, polyTimeComputable f
+  exists f, inhabited (polyTimeComputable f)
   /\ (forall x (Hx : vX x), {Hy : vY (f x) | (P (exist vX x Hx)) <-> (Q (exist vY (f x) Hy))}).
 Proof.
   intros [f ? ? ?]. eexists;split. easy.
@@ -150,11 +184,10 @@ Lemma reducesPolyMO_restriction_antimonotone X `{R :registered X} {vP} (P:restri
 Proof.
   intros f . 
   eapply reducesPolyMO_intro with (f := fun x => x). 2:easy.  
-  exists (fun _ => 1).
-  -constructor. extract. solverec.
-  -smpl_inO.
-  -hnf. reflexivity.
-  -exists (fun x => x). repeat split. 2-3:now smpl_inO.  reflexivity.
+  exists (fun _ => 1). 4:exists (fun x => x).
+  2,3,5,6:solve [ smpl_inO].
+  -extract. solverec.
+  -reflexivity.
 Qed.
 
 Lemma reducesPolyMO_reflexive X {regX : registered X} `(P : restrictedP vX) : P ⪯p P.
@@ -165,53 +198,49 @@ Qed.
 Lemma reducesPolyMO_transitive X Y Z {vX vY vZ} {regX : registered X} {regY : registered Y} {regZ : registered Z} (P : restrictedP (X:=X)vX) (Q : restrictedP (X:=Y)vY) (R : restrictedP (X:=Z)vZ) :
   P ⪯p Q -> Q ⪯p R -> P ⪯p R.
 Proof.
-  intros [f Cf Hf Hf'] [g Cg Hg Hg'].
+  intros [f f__c Hf Hf'] [g g__c Hg Hg'].
   eapply reducesPolyMO_intro with (f:= fun x =>g (f x)).
   2:{intros ?. eexists. now rewrite Hf',Hg'. 
   }
   clear dependent Hf. clear dependent Hg.
-  destruct Cf as [t__f [] ? f__mono (sizef&H__sizef&?&?)], Cg as [t__g [] ? g__mono (size__g&?&?&?)].
-  exists (fun x => t__f x + t__g (sizef x) + 1).
-  -split. extract. solverec.
-   hnf in g__mono.
-   erewrite g__mono. 2:eapply H__sizef. reflexivity.
+  (*destruct Cf as [t__f ? ? f__mono (sizef&H__sizef&?&?)] , Cg as [t__g ? ? g__mono (size__g&?&?&?)]. *)
+  exists (fun x => time__polyTC f__c x + time__polyTC g__c (resSize__rSP f__c x) + 1).
+  -extract. solverec.
+   erewrite (mono__polyTC g__c). 2:now apply bounds__rSP . reflexivity.
+  -smpl_inO.  eapply inOPoly_comp. all:smpl_inO.
   -smpl_inO.
-   eapply inOPoly_comp. all:smpl_inO.
-  -smpl_inO.
-  -exists (fun x => size__g (sizef x)). repeat split.
-   +intros. rewrite H1. hnf in H3;rewrite H3. 2:eapply H__sizef. reflexivity.
-   +eapply inOPoly_comp. all:try eassumption.
-   +eapply monotonic_comp. all:try eassumption.
+  -exists (fun x => resSize__rSP g__c (resSize__rSP f__c x)).
+   +intros. rewrite (bounds__rSP g__c), (mono__rSP g__c). 2:apply (bounds__rSP f__c). easy.
+   +eapply inOPoly_comp. all:smpl_inO.
+   +eapply monotonic_comp. all:smpl_inO.
 Qed.
 
 Lemma red_inNP X Y `{regX : registered X} `{regY : registered Y} `(P : restrictedP (X:=X) vX) `(Q : restrictedP (X:=Y) vY) :
   P ⪯p Q -> inNP Q -> inNP P.
 Proof.
-  intros [f Cf Hf] [R polyR certR]. 
+  intros [f f__comp Hf] [R polyR certR]. 
   unshelve eexists (fun '(exist _ x Hx) z => R (exist vY _ _) z). 1,2:easy. 
-  -destruct Cf as [? [] ? ? (fs&H__fs&?&mono__fs)].
-   destruct polyR as (f'__t&[f' [comp__f'] H__f']&?&mono_f'__t). 
-   eexists (fun n => polyTimeC__t n + f'__t (fs n + n) + 7). split.
-   +exists (fun '(x,z)=> f' (f x,z)).
-    split.
+  -(* destruct (polyRes__polyTC f__comp) as (size__f&Hsize__f&?&mono__sizef). *)
+   destruct polyR as (time__R&[R__comp]&inO__timeR&mono__timeR).
+   evar (time : nat -> nat). [time]:intros n.
+   exists time. split.
+   (*eexists (fun n => cnst n (*)polyTimeC__t n*) + time__R (time__polyTC f__comp (size__f n + n)) + 7). split.*)
+   +split. exists (fun '(x,z)=> f__decInTime R__comp (f x,z)).
     *extract. solverec.
-     all:rewrite !LProd.size_prod. all:cbn [fst snd].
-     hnf in polyTimeC__mono,mono_f'__t,mono__fs.
-     rewrite polyTimeC__mono with (x':=size (enc a) + size (enc b) + 4). 2:easy.
-     erewrite mono_f'__t with (x':=_). reflexivity.
-     rewrite H__fs.
-     rewrite mono__fs with (x':=(size (enc a) + size (enc b) + 4)). all:Lia.nia.
-    *intros [x c] Hx. specialize (H__f' (f x,c) (Hf _ Hx)). now cbn in *.  
-   +split.
-    all:smpl_inO.
+     all:rewrite !LProd.size_prod. all:cbn [fst snd]. set (n0:=size (enc a) + size (enc b) + 4).
+     rewrite (mono__polyTC _ (x':=n0)). 2:subst n0;nia.
+     erewrite (mono__timeR _ _).
+     2:{ rewrite (bounds__rSP f__comp), (mono__rSP f__comp (x':=n0)). 2:unfold n0;lia. instantiate (1:=resSize__rSP f__comp n0 + n0). unfold n0;try lia. }
+     unfold time. reflexivity. 
+    *intros [x c] Hx. cbn. rewrite <- correct__decInTime;cbn. easy.   
+   +unfold time;split;smpl_inO.
     { eapply inOPoly_comp. all:smpl_inO. }
-  -destruct certR as [? ? ? ? ?].
-   destruct Cf as [? ? ? ? (fs&H__fs&?&mono__fs)]. cbn.
-   exists (fun x =>  p (fs x)). 
-   +intros [] ? ?%polyCertRel_sound0;cbn. now apply f__correct.
-   +intros [] Hx;cbn. apply f__correct in Hx. edestruct polyCertRel_complete as (?&?&?). eauto. eexists;split. easy.
-    rewrite H1. cbn. apply mono__p. apply H__fs.
-   +now apply inOPoly_comp.
+  -clear - certR f__correct f__comp.
+   exists (fun x =>  p__pCR certR (resSize__rSP f__comp x)). 
+   +intros [] ? ?%(sound__pCR certR);cbn. now apply f__correct.
+   +intros [] Hx;cbn. apply f__correct in Hx. edestruct (complete__pCR certR) as (?&?&?). eauto. eexists;split. easy.
+    rewrite H0. cbn. apply mono__pCR. apply bounds__rSP.
+   +apply inOPoly_comp;smpl_inO.
    +smpl_inO.
 Qed.
 
