theories/L/Tactics/Computable.v
@@ -64,13 +64,12 @@ Class computable X {ty : TT X} (x : X) : Type :=
     extCorrect : computes ty x ext;
   }.
 
-Hint Mode computable + - +: typeclass_instances. (* treat argument as input and force evar-freeness*)
-
-Existing Instance ext | 5.
-
 Global Arguments computable {X} {ty} x.
 Global Arguments extCorrect {X} ty x {computable} : simpl never.
 Global Arguments ext {X} {ty} x {computable} : simpl never.
+
+Hint Mode computable + + +: typeclass_instances. (* treat argument as input and force evar-freeness*)
+Hint Extern 4 (@extracted ?t ?f) => let ty := constr:(_ : TT t) in notypeclasses refine (ext (ty:=ty) f) : typeclass_instances.
 
 Typeclasses Opaque ext.
 
